prove many properties about substitution, including the subtitution property of provability
this commit adds mathlib as dependency

language_term_n2.lean
@@ -6,8 +6,24 @@
 * There is no well-formedness predicate; all elements of type "term" are well-formed.
 -/
 
--- depend on mathlib
---import data.list.basic
+-- this file depends on mathlib
+import data.list.basic algebra.ordered_group
+
+namespace nat
+lemma add_sub_swap {n k : ℕ} (h : k ≤ n) (m : ℕ) : n + m - k = n - k + m :=
+by rw [add_comm, nat.add_sub_assoc h, add_comm]
+
+lemma one_le_of_lt {n k : ℕ} (H : n < k) : 1 ≤ k :=
+succ_le_of_lt (lt_of_le_of_lt n.zero_le H)
+
+lemma add_sub_cancel_right (n m k : ℕ) : n + (m + k) - k = n + m :=
+by rw [nat.add_sub_assoc, nat.add_sub_cancel]; apply k.le_add_left
+
+end nat
+
+lemma {u} lt_by_cases {α : Type u} [linear_order α] (x y : α) {P : Prop}
+  (h₁ : x < y → P) (h₂ : x = y → P) (h₃ : y < x → P) : P :=
+or.elim (lt_trichotomy x y) h₁ (λh, or.elim h h₂ h₃)
 
 namespace tactic
 namespace interactive
@@ -15,20 +31,20 @@ meta def congr1 : tactic unit := congr_core
 end interactive
 end tactic
 
-open list
+open list nat
 namespace fol
 structure Language := 
 (relations : ℕ → Type) (functions : ℕ → Type)
 section
 parameter {L : Language}
 
-/- preterm n is a partially applied term. if applied to n terms, it becomes a term.
+/- preterm l is a partially applied term. if applied to n terms, it becomes a term.
 * Every element of preterm 0 is well typed. 
 * We use this encoding to avoid mutual or nested inductive types, since those are not too convenient to work with in Lean. -/
 inductive preterm : ℕ → Type 
 | var : ℕ → preterm 0
-| func : ∀ {n : nat}, L.functions n → preterm n
-| apply : ∀ {n : nat}, preterm (n + 1) → preterm 0 → preterm n
+| func : ∀ {l : nat}, L.functions l → preterm l
+| app : ∀ {l : nat}, preterm (l + 1) → preterm 0 → preterm l
 open preterm
 @[reducible] def term := preterm 0
 
@@ -36,111 +52,208 @@ prefix `&`:max := _root_.fol.preterm.var
 
 /- lift_term_at _ t n m raises variables in t which are at least m by n -/
 @[simp] def lift_term_at : ∀ {l}, preterm l → ℕ → ℕ → preterm l
-| _ &k            n m := if m ≤ k then &(k+n) else &k
-| _ (func f)      n m := func f
-| _ (apply t1 t2) n m := apply (lift_term_at t1 n m) (lift_term_at t2 n m)
+| _ &k          n m := if m ≤ k then &(k+n) else &k
+| _ (func f)    n m := func f
+| _ (app t1 t2) n m := app (lift_term_at t1 n m) (lift_term_at t2 n m)
 
-notation t ` ↑ `:100 n ` # `:100 m:100 := _root_.fol.lift_term_at t n m -- input ↑ with \upa
+notation t ` ↑ `:90 n ` # `:90 m:90 := _root_.fol.lift_term_at t n m -- input ↑ with \u or \upa
 
-def lift_term (t : term) (n : ℕ) : term := t ↑ n # 0
-def lift_term1 (t : term) : term := t ↑ 1 # 0
+@[reducible] def lift_term {l} (t : preterm l) (n : ℕ) : preterm l := t ↑ n # 0
+@[reducible] def lift_term1 (t : term) : term := t ↑ 1 # 0
 
 infix ` ↑↑ `:100 := _root_.fol.lift_term -- input ↑ with \upa
 postfix ` ↑1`:100 := _root_.fol.lift_term1 -- input ↑ with \upa
 
 lemma lift_term_at_inj : ∀ {l} {t t' : preterm l} {n m : ℕ}, t ↑ n # m = t' ↑ n # m → t = t'
 | _ &k &k' n m h := 
-  by by_cases h₁ : m ≤ k; by_cases h₂ : m ≤ k'; simp [h₁, h₂] at h; 
-     congr;[exact add_right_cancel h, skip, skip, assumption]; exfalso; try {apply h₁}; 
-     try {apply h₂}; subst h; apply le_trans (by assumption) (nat.le_add_right _ _)
-| _ &k (func f')              n m h := by by_cases h' : m ≤ k; simp [h'] at h; contradiction
-| _ &k (apply t1' t2')        n m h := by by_cases h' : m ≤ k; simp [h'] at h; contradiction
-| _ (func f) &k'              n m h := by by_cases h' : m ≤ k'; simp [h'] at h; contradiction
-| _ (func f) (func f')        n m h := h
-| _ (func f) (apply t1' t2')  n m h := by cases h
-| _ (apply t1 t2) &k'         n m h := by by_cases h' : m ≤ k'; simp [h'] at h; contradiction
-| _ (apply t1 t2) (func f')   n m h := by cases h
-| _ (apply t1 t2) (apply t1' t2') n m h := 
+  by by_cases h₁ : m ≤ k; by_cases h₂ : m ≤ k'; simp [h₁, h₂] at h;
+     congr;[assumption, skip, skip, assumption]; exfalso; try {apply h₁}; 
+     try {apply h₂}; subst h; apply le_trans (by assumption) (le_add_right _ _)
+| _ &k (func f')            n m h := by by_cases h' : m ≤ k; simp [h'] at h; contradiction
+| _ &k (app t1' t2')        n m h := by by_cases h' : m ≤ k; simp [h'] at h; contradiction
+| _ (func f) &k'            n m h := by by_cases h' : m ≤ k'; simp [h'] at h; contradiction
+| _ (func f) (func f')      n m h := h
+| _ (func f) (app t1' t2')  n m h := by cases h
+| _ (app t1 t2) &k'         n m h := by by_cases h' : m ≤ k'; simp [h'] at h; contradiction
+| _ (app t1 t2) (func f')   n m h := by cases h
+| _ (app t1 t2) (app t1' t2') n m h := 
   begin injection h, congr; apply lift_term_at_inj; assumption end
 
 @[simp] lemma lift_term_at_zero : ∀ {l} (t : preterm l) (m : ℕ), t ↑ 0 # m = t
-| _ &k            m := by simp
-| _ (func f)      m := by refl
-| _ (apply t1 t2) m := by dsimp; congr; apply lift_term_at_zero
+| _ &k          m := by simp
+| _ (func f)    m := by refl
+| _ (app t1 t2) m := by dsimp; congr; apply lift_term_at_zero
 
 /- the following lemmas simplify iterated lifts, depending on the size of m' -/
 lemma lift_term_at2_small : ∀ {l} (t : preterm l) (n n') {m m'}, m' ≤ m → 
   (t ↑ n # m) ↑ n' # m' = (t ↑ n' # m') ↑ n # (m + n')
-| _ &k            n n' m m' H := 
+| _ &k          n n' m m' H := 
   begin 
     by_cases h : m ≤ k,
     { have h₁ : m' ≤ k, from le_trans H h,
       have h₂ : m' ≤ k + n, from le_trans h₁ (k.le_add_right n),
-      have h₃ : m + n' ≤ k + n', from add_le_add_right h _,
-      simp [h, h₁, h₂, h₃, -add_assoc, -add_comm], simp },
+      simp [*, -add_assoc, -add_comm], simp },
     { have h₁ : ¬m + n' ≤ k + n', from λ h', h (le_of_add_le_add_right h'),
       have h₂ : ¬m + n' ≤ k, from λ h', h₁ (le_trans h' (k.le_add_right n')),
-      by_cases h' : m' ≤ k; simp [h, h', h₁, h₂, -add_comm, -add_assoc], }
+      by_cases h' : m' ≤ k; simp [*, -add_comm, -add_assoc], }
   end
-| _ (func f)      n n' m m' H := by refl
-| _ (apply t1 t2) n n' m m' H := 
+| _ (func f)    n n' m m' H := by refl
+| _ (app t1 t2) n n' m m' H := 
   begin dsimp; congr1; apply lift_term_at2_small; assumption end
 
-lemma lift_term_at2_medium : ∀ {l} (t : preterm l) (n n') {m m'}, m ≤ m' → m' ≤ m+n → 
+lemma lift_term_at2_medium : ∀ {l} {t : preterm l} {n n' m m'}, m ≤ m' → m' ≤ m+n → 
   (t ↑ n # m) ↑ n' # m' = t ↑ (n+n') # m
-| _ &k            n n' m m' H₁ H₂ := 
+| _ &k          n n' m m' H₁ H₂ := 
   begin 
     by_cases h : m ≤ k,
     { have h₁ : m' ≤ k + n, from le_trans H₂ (add_le_add_right h n),
-      simp [h, h₁, -add_comm], },
-    { simp[h, -add_assoc, -add_comm],
+      simp [*, -add_comm], },
+    { simp [h, -add_assoc, -add_comm],
       have h₁ : ¬m' ≤ k, from λ h', h (le_trans H₁ h'),
-      simp [h, h₁, -add_comm, -add_assoc] }
+      simp [*, -add_comm, -add_assoc] }
   end
-| _ (func f)      n n' m m' H₁ H₂ := by refl
-| _ (apply t1 t2) n n' m m' H₁ H₂ := 
+| _ (func f)    n n' m m' H₁ H₂ := by refl
+| _ (app t1 t2) n n' m m' H₁ H₂ := 
   begin dsimp; congr1; apply lift_term_at2_medium; assumption end
+
+lemma lift_term2_medium {l} {t : preterm l} {n n' m'} (h : m' ≤ n) :
+  (t ↑↑ n) ↑ n' # m' = t ↑↑ (n+n') :=
+lift_term_at2_medium m'.zero_le (by simp*)
 
 lemma lift_term_at2_eq {l} (t : preterm l) (n n' m : ℕ) : 
   (t ↑ n # m) ↑ n' # (m+n) = t ↑ (n+n') # m :=
-lift_term_at2_medium t n n' (m.le_add_right n) (le_refl _)
+lift_term_at2_medium (m.le_add_right n) (le_refl _)
 
-lemma lift_term_at2_large {l} (t : preterm l) (n n') {m m'} (H : m' ≥ m + n) : 
+lemma lift_term_at2_large {l} (t : preterm l) (n n') {m m'} (H : m + n ≤ m') : 
   (t ↑ n # m) ↑ n' # m' = (t ↑ n' # (m'-n)) ↑ n # m :=
 have H₁ : n ≤ m', from le_trans (n.le_add_left m) H,
-have H₂ : m ≤ m' - n, by rw [←nat.add_sub_cancel m n]; apply nat.sub_le_sub_right; exact H,
+have H₂ : m ≤ m' - n, from nat.le_sub_right_of_add_le H,
 begin rw fol.lift_term_at2_small t n' n H₂, rw [nat.sub_add_cancel], exact H₁ end
 
-/- substitute_term t s n substitutes s for (&n) and reduces the level of all variables above n by 1 -/
-@[simp] def substitute_term : ∀ {l}, preterm l → term → ℕ → preterm l
-| _ &k            s n := if k < n then &k else if n < k then &(k-1) else s
-| _ (func f)      s n := func f
-| _ (apply t1 t2) s n := apply (substitute_term t1 s n) (substitute_term t2 s n)
+/- subst_term t s n substitutes s for (&n) and reduces the level of all variables above n by 1 -/
+def subst_term : ∀ {l}, preterm l → term → ℕ → preterm l
+| _ &k          s n := if k < n then &k else if n < k then &(k-1) else s ↑↑ n
+| _ (func f)    s n := func f
+| _ (app t1 t2) s n := app (subst_term t1 s n) (subst_term t2 s n)
 
-notation t `[`:95 s ` // `:95 n `]`:0 := _root_.fol.substitute_term t s n
+notation t `[`:max s ` // `:95 n `]`:0 := _root_.fol.subst_term t s n
 
-@[simp] def substitute_term_var_eq (t : term) (n : ℕ) : &n[t // n] = t :=
-by simp [lt_irrefl]
+@[simp] lemma subst_term_var_lt (s : term) {k n : ℕ} (H : k < n) : &k[s // n] = &k :=
+by simp [subst_term, H]
 
-lemma substitute_term_lift_term' : ∀{l} (t : preterm l) (s : term) (n : ℕ), 
-  (lift_term_at t 1 n)[s // n] = t :=
-sorry
+@[simp] lemma subst_term_var_gt (s : term) {k n : ℕ} (H : n < k) : &k[s // n] = &(k-1) :=
+have h : ¬(k < n), from lt_asymm H,
+by simp [*, subst_term]
 
-@[simp] lemma substitute_term_lift_term (t s : term) : (lift_term1 t)[s // 0] = t :=
-substitute_term_lift_term' t s 0
+@[simp] lemma subst_term_var_eq (s : term) (n : ℕ) : &n[s // n] = s ↑ n # 0 :=
+by simp [subst_term, lt_irrefl]
 
-/- preformula n is a partially applied formula. if applied to n terms, it becomes a formula. 
+lemma subst_term_var0 (s : term) : &0[s // 0] = s := by simp
+
+@[simp] lemma subst_term_func {l} (f : L.functions l) (s : term) (n : ℕ) : 
+  (func f)[s // n] = func f :=
+by refl
+
+@[simp] lemma subst_term_app {l} (t₁ : preterm (l+1)) (t₂ s : term) (n : ℕ) : 
+  (app t₁ t₂)[s // n] = app (t₁[s // n]) (t₂[s // n]) :=
+by refl
+
+/- the following lemmas simplify first lifting and then substituting, depending on the size
+  of the substituted variable -/
+lemma lift_at_subst_term_large : ∀{l} (t : preterm l) (s : term) {n₁ n₂ m}, m ≤ n₁ →
+ (t ↑ n₂ # m)[s // n₁+n₂] = (t [s // n₁]) ↑ n₂ # m
+| _ &k          s n₁ n₂ m h :=
+  begin
+    apply lt_by_cases k n₁; intro h₂,
+    { have : k < n₁ + n₂, from lt_of_le_of_lt (k.le_add_right n₂) (by simp*),
+      by_cases m ≤ k; simp* },
+    { subst h₂, simp [*, lift_term2_medium] },
+    { have h₂ : m < k, by apply lt_of_le_of_lt; assumption,
+      have : m ≤ k - 1, from nat.le_sub_right_of_add_le (succ_le_of_lt h₂),
+      have : m ≤ k, from le_of_lt h₂,
+      have : 1 ≤ k, from one_le_of_lt h₂,
+      simp [*, nat.add_sub_swap this n₂, -add_assoc, -add_comm] }
+  end
+| _ (func f)    s n₁ n₂ m h := rfl
+| _ (app t1 t2) s n₁ n₂ m h := by simp*
+
+lemma lift_subst_term_large {l} (t : preterm l) (s : term) {n₁ n₂} :
+  (t ↑↑ n₂)[s // n₁+n₂] = (t [s // n₁]) ↑↑ n₂ :=
+lift_at_subst_term_large t s n₁.zero_le
+
+lemma lift_at_subst_term_medium : ∀{l} (t : preterm l) (s : term) {n₁ n₂ m}, m ≤ n₂ → 
+  n₂ ≤ m + n₁ → (t ↑ n₁+1 # m)[s // n₂] = t ↑ n₁ # m
+| _ &k          s n₁ n₂ m h₁ h₂ := 
+  begin 
+    by_cases h : m ≤ k,
+    { have h₂ : n₂ < k + (n₁ + 1), from lt_succ_of_le (le_trans h₂ (add_le_add_right h _)), 
+      simp [*, add_sub_cancel_right] },
+    { have h₂ : k < n₂, from lt_of_lt_of_le (lt_of_not_ge h) h₁, simp* }
+  end
+| _ (func f)    s n₁ n₂ m h₁ h₂ := rfl
+| _ (app t1 t2) s n₁ n₂ m h₁ h₂ := by simp*
+
+lemma lift_subst_term_medium {l} (t : preterm l) (s : term) {n₁ n₂} :
+  (t ↑↑ ((n₁ + n₂) + 1))[s // n₂] = t ↑↑ (n₁ + n₂) :=
+lift_at_subst_term_medium t s n₂.zero_le (by rw [zero_add]; exact n₂.le_add_left n₁)
+
+lemma lift_at_subst_term_eq {l} (t : preterm l) (s : term) (n : ℕ) : (t ↑ 1 # n)[s // n] = t :=
+begin rw [lift_at_subst_term_medium t s, lift_term_at_zero]; refl end
+
+@[simp] lemma lift_term1_subst_term (t s : term) : (lift_term1 t)[s // 0] = t :=
+lift_at_subst_term_eq t s 0
+
+lemma subst_term2 : ∀{l} (t : preterm l) (s₁ s₂ : term) (n₁ n₂),
+  t [s₁ // n₁] [s₂ // n₁ + n₂] = t [s₂ // n₁ + n₂ + 1] [s₁[s₂ // n₂] // n₁]
+| _ &k          s₁ s₂ n₁ n₂ :=
+  begin
+    apply lt_by_cases k n₁; intro h,
+    { have : k < n₁ + n₂, from lt_of_le_of_lt (k.le_add_right n₂) (by simp*),
+      have : k < n₁ + n₂ + 1, from lt.step this,
+      simp [*, -add_comm, -add_assoc] },
+    { have : k < k + (n₂ + 1), from lt_succ_of_le (le_add_right _ n₂),
+      subst h, simp [*, -add_comm], refine eq.trans _ (lift_subst_term_large _ _),
+      rw [add_comm] },
+    apply lt_by_cases k (n₁ + n₂ + 1); intro h',
+    { have : k - 1 < n₁ + n₂, from (nat.sub_lt_right_iff_lt_add (one_le_of_lt h)).2 h', 
+      simp [*, -add_comm, -add_assoc] },
+    { subst h', simp [h, -add_comm, -add_assoc], symmetry, apply lift_at_subst_term_medium,
+      apply n₁.zero_le, rw [zero_add], apply n₁.le_add_right },
+    { have : n₁ + n₂ < k - 1, from nat.lt_sub_right_of_add_lt h', 
+      have : n₁ < k - 1, from lt_of_le_of_lt (n₁.le_add_right n₂) this,
+      simp [*, -add_comm, -add_assoc] }
+  end
+| _ (func f)    s₁ s₂ n₁ n₂ := rfl
+| _ (app t1 t2) s₁ s₂ n₁ n₂ := by simp*
+
+
+lemma subst_term2_0 {l} (t : preterm l) (s₁ s₂ : term) (n) :
+  t [s₁ // 0] [s₂ // n] = t [s₂ // n + 1] [s₁[s₂ // n] // 0] :=
+let h := subst_term2 t s₁ s₂ 0 n in by simp at h; exact h
+
+/- Probably useful facts about substitution which we should add when needed:
+(forall M N i j k, ( M [ j ← N] ) ↑ k # (j+i) = (M ↑ k # (S (j+i))) [ j ← (N ↑ k # i ) ])
+
+
+subst_travers : (forall M N P n, (M [← N]) [n ← P] = (M [n+1 ← P])[← N[n← P]])
+erasure_lem1 : (forall a n, a = (a ↑ 1 # (S n)) [n ← #0])
+erasure_lem3 : (forall n m t, m>n->#m = (#m ↑ 1 # (S n)) [n ← t]). 
+lift_is_lift_sublemma : forall j v, j<v->exists w,#v=w↑1#j. 
+lift_is_lift : (forall N A n i j,N ↑ i # n=A ↑ 1 # j -> j<n -> exists M,N=M ↑ 1 # j)
+subst_is_lift : (forall N T A n j, N [n ← T]=A↑ 1#j->j<n->exists M,N=M↑ 1#j)
+-/
+
+/- preformula l is a partially applied formula. if applied to n terms, it becomes a formula. 
   * We only have implication as binary connective. Since we use classical logic, we can define
     the other connectives from implication and false. 
   * Similarly, universal quantification is our only quantifier. 
   * We could make `false` and `equal` into elements of rel. However, if we do that, then we cannot make the interpretation of them in a model definitionally what we want.
-
 -/
 inductive preformula : ℕ → Type 
 | false : preformula 0
 | equal : term → term → preformula 0
-| rel : ∀ {n : nat}, L.relations n → preformula n
-| apprel : ∀ {n : nat}, preformula (n + 1) → term → preformula n
+| rel : ∀ {l : nat}, L.relations l → preformula l
+| apprel : ∀ {l : nat}, preformula (l + 1) → term → preformula l
 | imp : preformula 0 → preformula 0 → preformula 0
 | all : preformula 0 → preformula 0
 open preformula
@@ -153,25 +266,33 @@ def iff (f₁ f₂ : formula) : formula := and (imp f₁ f₂) (imp f₂ f₁)
 def ex (f : formula) : formula := not (all (not f))
 
 notation `⊥` := _root_.fol.preformula.false -- input: \bot
-infix ` ≃ `:90 := _root_.fol.preformula.equal -- input \~- or \simeq
-infix ` ⟹ `:70 := _root_.fol.preformula.imp -- input \==>
-prefix `~` := _root_.fol.not
-infixr ` ⊔ `:80 := _root_.fol.or -- input: \sqcup
-infixr ` ⊓ `:85 := _root_.fol.and -- input: \sqcap
-
+infix ` ≃ `:88 := _root_.fol.preformula.equal -- input \~- or \simeq
+infix ` ⟹ `:62 := _root_.fol.preformula.imp -- input \==>
+prefix `∼`:max := _root_.fol.not -- input \~
+prefix [parsing_only] `~` := _root_.fol.not -- this is the ASCII character. warning: this has a way too low precedence. Use \~ for an operation with a good precedence.
+infixr ` ⊔ ` := _root_.fol.or -- input: \sqcup
+infixr ` ⊓ ` := _root_.fol.and -- input: \sqcap
+prefix `∀∀`:110 := _root_.fol.preformula.all
+prefix `∃∃`:110 := _root_.fol.ex
 
 @[simp] def lift_formula_at : ∀ {l}, preformula l → ℕ → ℕ → preformula l
 | _ false        n m := false
 | _ (t1 ≃ t2)    n m := equal (lift_term_at t1 n m) (lift_term_at t2 n m)
 | _ (rel R)      n m := rel R
 | _ (apprel f t) n m := apprel (lift_formula_at f n m) (lift_term_at t n m)
-| _ (imp f1 f2)  n m := imp (lift_formula_at f1 n m) (lift_formula_at f2 n m)
-| _ (all f)      n m := all (lift_formula_at f n (m+1))
+| _ (f1 ⟹ f2)   n m := lift_formula_at f1 n m ⟹ lift_formula_at f2 n m
+| _ (∀∀ f)       n m := ∀∀ lift_formula_at f n (m+1)
 
-notation f ` ↑ `:100 n ` # `:100 m:100 := _root_.fol.lift_formula_at f n m -- input ↑ with \upa
+notation f ` ↑ `:90 n ` # `:90 m:90 := _root_.fol.lift_formula_at f n m -- input ↑ with \upa
 
-def lift_formula (f : formula) (n : ℕ) : formula := f ↑ n # 0
-def lift_formula1 (f : formula) : formula := f ↑ 1 # 0
+@[reducible] def lift_formula {l} (f : preformula l) (n : ℕ) : preformula l := f ↑ n # 0
+@[reducible] def lift_formula1 (f : formula) : formula := f ↑ 1 # 0
+
+infix ` ↑↑ `:100 := _root_.fol.lift_formula -- input ↑ with \upa
+postfix ` ↑1`:100 := _root_.fol.lift_formula1 -- input ↑ with \upa
+
+@[simp] lemma lift_formula1_not (f : formula) : lift_formula1 (not f) = not (lift_formula1 f) :=
+by refl
 
 lemma lift_formula_at_inj {l} {f f' : preformula l} {n m : ℕ} (H : f ↑ n # m = f' ↑ n # m) : f = f' :=
 begin
@@ -187,8 +308,8 @@ end
 | _ (t1 ≃ t2)    m := by simp
 | _ (rel R)      m := by refl
 | _ (apprel f t) m := by simp; apply lift_formula_at_zero
-| _ (imp f1 f2)  m := by dsimp; congr1; apply lift_formula_at_zero
-| _ (all f)      m := by simp; apply lift_formula_at_zero
+| _ (f1 ⟹ f2)   m := by dsimp; congr1; apply lift_formula_at_zero
+| _ (∀∀ f)       m := by simp; apply lift_formula_at_zero
 
 /- the following lemmas simplify iterated lifts, depending on the size of m' -/
 lemma lift_formula_at2_small : ∀ {l} (f : preformula l) (n n') {m m'}, m' ≤ m → 
@@ -198,21 +319,19 @@ lemma lift_formula_at2_small : ∀ {l} (f : preformula l) (n n') {m m'}, m' ≤ 
 | _ (rel R)      n n' m m' H := by refl
 | _ (apprel f t) n n' m m' H := 
   by simp [lift_term_at2_small, H, -add_comm]; apply lift_formula_at2_small; assumption
-| _ (imp f1 f2)  n n' m m' H := by dsimp; congr1; apply lift_formula_at2_small; assumption
-| _ (all f)      n n' m m' H :=
+| _ (f1 ⟹ f2)   n n' m m' H := by dsimp; congr1; apply lift_formula_at2_small; assumption
+| _ (∀∀ f)       n n' m m' H :=
   by simp [lift_term_at2_small, H, lift_formula_at2_small f n n' (add_le_add_right H 1)]
 
 lemma lift_formula_at2_medium : ∀ {l} (f : preformula l) (n n') {m m'}, m ≤ m' → m' ≤ m+n → 
   (f ↑ n # m) ↑ n' # m' = f ↑ (n+n') # m
 | _ false        n n' m m' H₁ H₂ := by refl
-| _ (t1 ≃ t2)    n n' m m' H₁ H₂ := by simp [lift_term_at2_medium, H₁, H₂]
+| _ (t1 ≃ t2)    n n' m m' H₁ H₂ := by simp [*, lift_term_at2_medium]
 | _ (rel R)      n n' m m' H₁ H₂ := by refl
-| _ (apprel f t) n n' m m' H₁ H₂ :=
-  by simp [lift_term_at2_medium, H₁, H₂, -add_comm]; apply lift_formula_at2_medium; assumption
-| _ (imp f1 f2)  n n' m m' H₁ H₂ := by dsimp; congr1; apply lift_formula_at2_medium; assumption
-| _ (all f)      n n' m m' H₁ H₂ :=
-  have m' + 1 ≤ (m + 1) + n, from le_trans (add_le_add_right H₂ 1) (by simp),
-  by simp [lift_term_at2_medium, H₁, H₂, lift_formula_at2_medium f n n' (add_le_add_right H₁ 1) this]
+| _ (apprel f t) n n' m m' H₁ H₂ := by simp [*, lift_term_at2_medium, -add_comm]
+| _ (f1 ⟹ f2)   n n' m m' H₁ H₂ := by simp*
+| _ (∀∀ f)       n n' m m' H₁ H₂ :=
+  have m' + 1 ≤ (m + 1) + n, from le_trans (add_le_add_right H₂ 1) (by simp), by simp*
 
 lemma lift_formula_at2_eq {l} (f : preformula l) (n n' m : ℕ) : 
   (f ↑ n # m) ↑ n' # (m+n) = f ↑ (n+n') # m :=
@@ -221,24 +340,52 @@ lift_formula_at2_medium f n n' (m.le_add_right n) (le_refl _)
 lemma lift_formula_at2_large {l} (f : preformula l) (n n') {m m'} (H : m' ≥ m + n) : 
   (f ↑ n # m) ↑ n' # m' = (f ↑ n' # (m'-n)) ↑ n # m :=
 have H₁ : n ≤ m', from le_trans (n.le_add_left m) H,
-have H₂ : m ≤ m' - n, by rw [←nat.add_sub_cancel m n]; apply nat.sub_le_sub_right; exact H,
+have H₂ : m ≤ m' - n, from nat.le_sub_right_of_add_le H,
 begin rw fol.lift_formula_at2_small f n' n H₂, rw [nat.sub_add_cancel], exact H₁ end
 
-@[simp] def substitute_formula : ∀ {l}, preformula l → term → ℕ → preformula l
+@[simp] def subst_formula : ∀ {l}, preformula l → term → ℕ → preformula l
 | _ false        s n := false
-| _ (t1 ≃ t2)    s n := equal (substitute_term t1 s n) (substitute_term t2 s n)
+| _ (t1 ≃ t2)    s n := subst_term t1 s n ≃ subst_term t2 s n
 | _ (rel R)      s n := rel R
-| _ (apprel f t) s n := apprel (substitute_formula f s n) (substitute_term t s n)
-| _ (imp f1 f2)  s n := imp (substitute_formula f1 s n) (substitute_formula f2 s n)
-| _ (all f)      s n := all (substitute_formula f s (n+1))
+| _ (apprel f t) s n := apprel (subst_formula f s n) (subst_term t s n)
+| _ (f1 ⟹ f2)   s n := subst_formula f1 s n ⟹ subst_formula f2 s n
+| _ (∀∀ f)       s n := ∀∀ subst_formula f s (n+1)
 
-notation f `[`:95 s ` // `:95 n `]`:0 := _root_.fol.substitute_formula f s n
+notation f `[`:95 s ` // `:95 n `]`:0 := _root_.fol.subst_formula f s n
 
-@[simp] def substitute_formula_equal (t₁ t₂ s : term) (n : ℕ) :
+lemma subst_formula_equal (t₁ t₂ s : term) (n : ℕ) :
   (t₁ ≃ t₂)[s // n] = t₁[s // n] ≃ (t₂[s // n]) :=
-by refl
+by simp
 
--- ⟹⇔≃
+/- this lemma is in the other directions as similar lemma's, because only in this direction
+  simp* can do the `all` case, and I'm lazy. -/
+lemma lift_at_subst_formula_large' : ∀{l} (f : preformula l) (s : term) {n₁ n₂ m}, m ≤ n₁ →
+  (f [s // n₁]) ↑ n₂ # m = (f ↑ n₂ # m)[s // n₁+n₂]
+| _ false        s n₁ n₂ m h := by refl
+| _ (t1 ≃ t2)    s n₁ n₂ m h := by simp [*, lift_at_subst_term_large]
+| _ (rel R)      s n₁ n₂ m h := by refl
+| _ (apprel f t) s n₁ n₂ m h := by simp [*, lift_at_subst_term_large]
+| _ (f1 ⟹ f2)   s n₁ n₂ m h := by simp*
+| _ (∀∀ f)       s n₁ n₂ m h := by simp*
+
+lemma lift_subst_formula_large {l} (f : preformula l) (s : term) {n₁ n₂} :
+ (f ↑↑ n₂)[s // n₁+n₂] = (f [s // n₁]) ↑↑ n₂ :=
+(lift_at_subst_formula_large' f s n₁.zero_le).symm
+
+lemma subst_formula2 : ∀{l} (f : preformula l) (s₁ s₂ : term) (n₁ n₂),
+  f [s₁ // n₁] [s₂ // n₁ + n₂] = f [s₂ // n₁ + n₂ + 1] [s₁[s₂ // n₂] // n₁]
+| _ false        s₁ s₂ n₁ n₂ := by refl
+| _ (t1 ≃ t2)    s₁ s₂ n₁ n₂ := by simp [*, subst_term2]
+| _ (rel R)      s₁ s₂ n₁ n₂ := by refl
+| _ (apprel f t) s₁ s₂ n₁ n₂ := by simp [*, subst_term2]
+| _ (f1 ⟹ f2)   s₁ s₂ n₁ n₂ := by simp*
+| _ (∀∀ f)       s₁ s₂ n₁ n₂ := 
+  by simp*; rw [add_comm n₂ 1, ←add_assoc, subst_formula2 f s₁ s₂ (n₁ + 1) n₂]; simp
+
+lemma subst_formula2_zero {l} (f : preformula l) (s₁ s₂ : term) (n) :
+  f [s₁ // 0] [s₂ // n] = f [s₂ // n + 1] [s₁[s₂ // n] // 0] :=
+let h := subst_formula2 f s₁ s₂ 0 n in by simp at h; exact h
+
 /- Provability relation
 * to decide: should Γ be a list or a set (or finset)?
 * We use natural deduction as our deduction system, since that is most convenient to work with.
@@ -248,34 +395,15 @@ inductive prf : list formula → formula → Type
 | axm    : ∀{Γ A}, A ∈ Γ → prf Γ A
 | impI   : ∀{Γ A B}, prf (A::Γ) B → prf Γ (A ⟹ B)
 | impE   : ∀{Γ} (A) {B}, prf Γ (A ⟹ B) → prf Γ A → prf Γ B
-| falseE : ∀{Γ A}, prf (not A::Γ) false → prf Γ A
-| allI   : ∀{Γ A}, prf (map lift_formula1 Γ) A → prf Γ (all A)
-| allE'  : ∀{Γ} A t, prf Γ (all A) → prf Γ (A[t // 0])
+| falseE : ∀{Γ A}, prf (∼A::Γ) false → prf Γ A
+| allI   : ∀{Γ A}, prf (map lift_formula1 Γ) A → prf Γ (∀∀ A)
+| allE'  : ∀{Γ} A t, prf Γ (∀∀ A) → prf Γ (A[t // 0])
 | refl   : ∀Γ t, prf Γ (t ≃ t)
 | subst' : ∀{Γ} s t f, prf Γ (s ≃ t) → prf Γ (f[s // 0]) → prf Γ (f[t // 0])
 open prf
 infix ` ⊢ `:51 := _root_.fol.prf -- input: \|- or \vdash
 
-def weakening {Γ Δ} {f : formula} (H₁ : Γ ⊆ Δ) (H₂ : Γ ⊢ f) : Δ ⊢ f :=
-begin
-  induction H₂ generalizing Δ,
-  { apply axm, exact H₁ H₂_a, },
-  { apply impI, apply H₂_ih, simp [cons_subset_cons, H₁] },
-  { apply impE, apply H₂_ih_a, assumption, apply H₂_ih_a_1, assumption },
-  { apply falseE, apply H₂_ih, simp [cons_subset_cons, H₁] },
-  { apply allI, apply H₂_ih, sorry /-simp [cons_subset_cons, H₁]-/ },
-  { apply allE', apply H₂_ih, assumption },
-  { apply refl },
-  { apply subst', apply H₂_ih_a, assumption, apply H₂_ih_a_1, assumption },
-end
-
-def weakening_cons {Γ} {f₁ f₂ : formula} (H : Γ ⊢ f₂) : f₁::Γ ⊢ f₂ :=
-weakening (Γ.subset_cons f₁) H
-
-def weakening_cons2 {Γ} {f₁ f₂ f₃ : formula} (H : f₁::Γ ⊢ f₂) : f₁::f₃::Γ ⊢ f₂ :=
-weakening (cons_subset_cons _ (Γ.subset_cons _)) H
-
-def allE {Γ} (A : formula) (t) {B} (H₁ : prf Γ (all A)) (H₂ : A[t // 0] = B) : prf Γ B :=
+def allE {Γ} (A : formula) (t) {B} (H₁ : prf Γ (∀∀ A)) (H₂ : A[t // 0] = B) : prf Γ B :=
 by induction H₂; exact allE' A t H₁
 
 def subst {Γ} {s t} (f₁ : formula) {f₂} (H₁ : prf Γ (s ≃ t)) (H₂ : prf Γ (f₁[s // 0])) 
@@ -285,44 +413,75 @@ by induction H₃; exact subst' s t f₁ H₁ H₂
 def axm1 {Γ} {A : formula} : A::Γ ⊢ A := by apply axm; left; refl
 def axm2 {Γ} {A B : formula} : A::B::Γ ⊢ B := by apply axm; right; left; refl
 
+def weakening {Γ Δ} {f : formula} (H₁ : Γ ⊆ Δ) (H₂ : Γ ⊢ f) : Δ ⊢ f :=
+begin
+  induction H₂ generalizing Δ,
+  { apply axm, exact H₁ H₂_a, },
+  { apply impI, apply H₂_ih, simp [cons_subset_cons, H₁] },
+  { apply impE, apply H₂_ih_a, assumption, apply H₂_ih_a_1, assumption },
+  { apply falseE, apply H₂_ih, simp [cons_subset_cons, H₁] },
+  { apply allI, apply H₂_ih, apply map_subset _ H₁ },
+  { apply allE', apply H₂_ih, assumption },
+  { apply refl },
+  { apply subst', apply H₂_ih_a, assumption, apply H₂_ih_a_1, assumption },
+end
+
+def substitution {Γ} {f : formula} {t n} (H : Γ ⊢ f) : map (λx, x[t // n]) Γ ⊢ f[t // n] :=
+begin
+  induction H generalizing n,
+  { apply axm, apply mem_map_of_mem _ H_a, },
+  { apply impI, apply H_ih },
+  { apply impE, apply H_ih_a, apply H_ih_a_1 },
+  { apply falseE, apply H_ih },
+  { apply allI, rw list.map_map, have h := @H_ih (n+1), rw list.map_map at h, 
+    apply cast _ h, congr1; [skip, refl], apply map_congr, intros,
+    apply lift_subst_formula_large },
+  { apply allE _ _ H_ih, symmetry, apply subst_formula2_zero },
+  { apply refl },
+  { apply subst _ H_ih_a, { have h := @H_ih_a_1 n, rw [subst_formula2_zero] at h, exact h}, 
+    rw [subst_formula2_zero] },
+end
+
+def weakening1 {Γ} {f₁ f₂ : formula} (H : Γ ⊢ f₂) : f₁::Γ ⊢ f₂ :=
+weakening (Γ.subset_cons f₁) H
+
+def weakening2 {Γ} {f₁ f₂ f₃ : formula} (H : f₁::Γ ⊢ f₂) : f₁::f₃::Γ ⊢ f₂ :=
+weakening (cons_subset_cons _ (Γ.subset_cons _)) H
+
 def deduction {Γ} {A B : formula} (H : Γ ⊢ A ⟹ B) : A::Γ ⊢ B :=
-impE A (weakening_cons H) axm1
+impE A (weakening1 H) axm1
 
 def exfalso {Γ} {A : formula} (H : prf Γ false) : prf Γ A :=
-falseE (weakening_cons H)
+falseE (weakening1 H)
 
 def andI {Γ} {f₁ f₂ : formula} (H₁ : Γ ⊢ f₁) (H₂ : Γ ⊢ f₂) : Γ ⊢ f₁ ⊓ f₂ :=
 begin 
   apply impI, apply impE f₂,
-  { apply impE f₁, apply axm1, exact weakening_cons H₁ },
-  { exact weakening_cons H₂ }
+  { apply impE f₁, apply axm1, exact weakening1 H₁ },
+  { exact weakening1 H₂ }
 end
 
 def andE1 {Γ f₁} (f₂ : formula) (H : Γ ⊢ f₁ ⊓ f₂) : Γ ⊢ f₁ :=
 begin 
-  apply falseE, apply impE _ (weakening_cons H), apply impI, apply exfalso,
+  apply falseE, apply impE _ (weakening1 H), apply impI, apply exfalso,
   apply impE f₁; [apply axm2, apply axm1]
 end
 
 def andE2 {Γ} (f₁ : formula) {f₂} (H : Γ ⊢ f₁ ⊓ f₂) : Γ ⊢ f₂ :=
-begin 
-  apply falseE, apply impE _ (weakening_cons H), apply impI, apply axm2
-end
+begin apply falseE, apply impE _ (weakening1 H), apply impI, apply axm2 end
 
 def orI1 {Γ} {A B : formula} (H : Γ ⊢ A) : Γ ⊢ A ⊔ B :=
-begin
-  apply impI, apply exfalso, refine impE _ _ (weakening_cons H), apply axm1
-end
+begin apply impI, apply exfalso, refine impE _ _ (weakening1 H), apply axm1 end
 
 def orI2 {Γ} {A B : formula} (H : Γ ⊢ B) : Γ ⊢ A ⊔ B :=
-impI $ weakening_cons H
+impI $ weakening1 H
 
 def orE {Γ} {A B C : formula} (H₁ : Γ ⊢ A ⊔ B) (H₂ : A::Γ ⊢ C) (H₃ : B::Γ ⊢ C) : Γ ⊢ C :=
 begin
   apply falseE, apply impE C, { apply axm1 },
-  apply impE B, { apply impI, exact weakening_cons2 H₃ },
-  apply impE _ (weakening_cons H₁),
-  apply impI (impE _ axm2 (weakening_cons2 H₂))
+  apply impE B, { apply impI, exact weakening2 H₃ },
+  apply impE _ (weakening1 H₁),
+  apply impI (impE _ axm2 (weakening2 H₂))
 end
 
 def iffI {Γ} {f₁ f₂ : formula} (H₁ : f₁::Γ ⊢ f₂) (H₂ : f₂::Γ ⊢ f₁) : Γ ⊢ iff f₁ f₂ :=
@@ -334,27 +493,37 @@ deduction (andE1 _ H)
 def iffE2 {Γ} {f₁ f₂ : formula} (H : Γ ⊢ iff f₁ f₂) : f₂::Γ ⊢ f₁ :=
 deduction (andE2 _ H)
 
--- def ex (f : formula) : formula := not (all (not f))
+def exI {Γ f} (t : term) (H : Γ ⊢ f [t // 0]) : Γ ⊢ ∃∃ f :=
+begin
+  apply impI, 
+  apply impE (f[t // 0]) _ (weakening1 H),
+  apply allE' ∼f t axm1,
+end
+
+def exE {Γ f₁ f₂} (t : term) (H₁ : Γ ⊢ ∃∃ f₁) (H₂ : f₁::map lift_formula1 Γ ⊢ lift_formula1 f₂) :
+  Γ ⊢ f₂ :=
+begin
+  apply falseE, apply impE _ (weakening1 H₁), apply allI, apply impI, 
+  apply impE _ axm2, apply weakening2 H₂
+end
 
 def symm {Γ} {s t : term} (H : Γ ⊢ s ≃ t) : Γ ⊢ t ≃ s :=
 begin 
-  apply subst (&0 ≃ s ↑1) H; 
-    rw [substitute_formula_equal, substitute_term_lift_term, substitute_term_var_eq],
+  apply subst (&0 ≃ s ↑1) H; rw [subst_formula_equal, lift_term1_subst_term, subst_term_var0],
   apply refl
 end
 
 def trans {Γ} {t₁ t₂ t₃ : term} (H : Γ ⊢ t₁ ≃ t₂) (H' : Γ ⊢ t₂ ≃ t₃) : Γ ⊢ t₁ ≃ t₃ :=
 begin 
-  apply subst (t₁ ↑1 ≃ &0) H';
-    rw [substitute_formula_equal, substitute_term_lift_term, substitute_term_var_eq],
+  apply subst (t₁ ↑1 ≃ &0) H'; rw [subst_formula_equal, lift_term1_subst_term, subst_term_var0],
   exact H
 end
 
 def congr {Γ} {t₁ t₂ s : term} (H : Γ ⊢ t₁ ≃ t₂) : Γ ⊢ s[t₁ // 0] ≃ s[t₂ // 0] :=
 begin 
   apply subst (s[t₁ // 0] ↑1 ≃ s) H, 
-  { rw [substitute_formula_equal, substitute_term_lift_term], apply refl },
-  { rw [substitute_formula_equal, substitute_term_lift_term] }
+  { rw [subst_formula_equal, lift_term1_subst_term], apply refl },
+  { rw [subst_formula_equal, lift_term1_subst_term] }
 end
 
 end
